\documentclass{article}
\usepackage{graphicx}
\usepackage{amsmath}
\begin{document}
	\begin{equation}
	k! \ge (\frac{k}{e})^k
	\end{equation}
	\begin{equation}
	e^k = 1 + \frac{k}{1!} + \frac{k^2}{2!} + \frac{k^3}{3!} + \frac{k^4}{4!} + ... + \frac{k^k}{k!} + ...
	\end{equation}
	\begin{equation}
	k!e^k = k!(1 + \frac{k}{1!} + \frac{k^2}{2!} + \frac{k^3}{3!} + \frac{k^4}{4!} + ... + \frac{k^k}{k!} + ...)
	\end{equation}
	\begin{equation}
	k!e^k = k! + k!\frac{k}{1!} + k!\frac{k^2}{2!} + k!\frac{k^3}{3!} + k!\frac{k^4}{4!} + ... + k!\frac{k^k}{k!} + ...
	\end{equation}
	\begin{equation}
	k!e^k = k! + k!\frac{k}{1!} + k!\frac{k^2}{2!} + k!\frac{k^3}{3!} + k!\frac{k^4}{4!} + ... + k^k + ...
	\end{equation}
	\begin{equation}
	k!e^k = k^k + \Delta
	\end{equation}
	\begin{equation}
	k!e^k \ge k^k
	\end{equation}
	\begin{equation}
	k! \ge \frac{k^k}{e^k}
	\end{equation}
	\begin{equation}
	k! \ge (\frac{k}{e})^k
	\end{equation}
	\begin{equation}
	{n \choose k} = \frac{n!}{k!(n - k)!}
	\end{equation}
\end{document}