\documentclass{article}
\usepackage{graphicx}
\usepackage{amsmath}
\begin{document}
	\begin{equation}
	S = 0 + q + 2q^2 + 3q^3 + 4q^4 + ...
	\end{equation}
	\begin{equation}
	S = q(1 + 2q + 3q^2 + 4q^3 + ...)
	\end{equation}
	\begin{equation}
	S = q(1 + q + 2q^2 + 3q^3 + ... + q + q^2 + q^3 + ....)
	\end{equation}
	\begin{equation}
	S = q(S + \frac{1}{1 - q})
	\end{equation}
	\begin{equation}
	S = qS + \frac{q}{1 - q}
	\end{equation}
	\begin{equation}
	S - qS = \frac{q}{1 - q}
	\end{equation}
	\begin{equation}
	S(1 - q) = \frac{q}{1 - q}
	\end{equation}
	\begin{equation}
	S = \frac{q}{(1 - q)^2}
	\end{equation}
\end{document}